code/frodo/Hacl.Impl.Frodo.Params.fst
@@ -1,7 +1,7 @@
 module Hacl.Impl.Frodo.Params
 
 open Lib.IntTypes
-open Lib.Buffer
+open Lib.PQ.Buffer
 
 let params_n = size 64
 
@@ -13,8 +13,8 @@ let crypto_bytes = size 16
 
 let cdf_table_len = size 12
 
-let cdf_table =
-  gcmalloc_of_list HyperStack.root
+let cdf_table: b:lbuffer uint16 (v cdf_table_len) { LowStar.Buffer.recallable b } =
+  LowStar.Buffer.gcmalloc_of_list HyperStack.root
     [u16 4727; u16 13584; u16 20864; u16 26113; u16 29434; u16 31278;
      u16 32176; u16 32560; u16 32704; u16 32751; u16 32764; u16 32767]
 
